\documentclass[12pt]{article}
\usepackage{amsmath}
\usepackage{times}
\usepackage{anyfontsize}
\usepackage{amsfonts}
\usepackage{mathtools}
\usepackage[paperheight=6in,paperwidth=6in,margin=0.6in]{geometry}
\usepackage[x11names]{xcolor}
\usepackage{tikz}
\usepackage{tcolorbox}
\setlength{\parindent}{0cm}
\usepackage{graphicx}
\usepackage{background}
\usepackage{blindtext}
\backgroundsetup{ scale=1, angle=0, opacity=1, contents={\begin{tikzpicture}[remember picture,overlay] \path [left color=LightSkyBlue1, right color=white] (current page.south west)rectangle (current page.north east);  
\end{tikzpicture}} }
\graphicspath{{images/}}
\setcounter{section}{1}
\pagestyle{empty}
\begin{document}
\color{black}
\pagebreak

\section{Proof:-}

Let $A=a_1+a_2+\cdots+a_n;$ $B=b_1+b_2+\cdots+b_n; $ $\cdots \cdots;$ $L=l_1+l_2+\cdots+l _n $

Consider the positive numbers $\dfrac{a_1}{A},\dfrac{b_1}{B},\cdots, \dfrac{l_1}{L}$ with associative positive rational weights $\alpha,\beta,\cdots,\lambda $ respectively. Then $$\alpha\bigg(\dfrac{a_1}{A}\bigg)+\beta\bigg(\dfrac{b_1}{B}\bigg)+\cdots+\lambda\bigg(\dfrac{l_1}{L}\bigg)\geq \bigg(\dfrac{a_1}{A}\bigg)^{\alpha}\bigg(\dfrac{b_1}{B}\bigg)^{\beta}\cdots\bigg(\dfrac{l_1}{L}\bigg)^{\lambda}$$Similarly $$\alpha\bigg(\dfrac{a_2}{A}\bigg)+\beta\bigg(\dfrac{b_2}{B}\bigg)+\cdots+\lambda\bigg(\dfrac{l_2}{L}\bigg)\geq \bigg(\dfrac{a_2}{A}\bigg)^{\alpha}\bigg(\dfrac{b_2}{B}\bigg)^{\beta}\cdots\bigg(\dfrac{l_2}{L}\bigg)^{\lambda}$$ $$\vdots\qquad\qquad\qquad\qquad \vdots \qquad\qquad\qquad\qquad \vdots$$ $$\alpha\bigg(\dfrac{a_n}{A}\bigg)+\beta\bigg(\dfrac{b_n}{B}\bigg)+\cdots+\lambda\bigg(\dfrac{l_n}{L}\bigg)\geq \bigg(\dfrac{a_n}{A}\bigg)^{\alpha}\bigg(\dfrac{b_n}{B}\bigg)^{\beta}\cdots\bigg(\dfrac{l_n}{L}\bigg)^{\lambda}$$
\pagebreak 

Therefore
 $$\displaystyle{\frac{\splitdfrac{\left(\frac{a_1}{A}\right)^{\alpha}\left(\frac{b_1}{B}\right)^{\beta}\cdots\left(\frac{l_1}{L}\right)^{\lambda} +  \left(\frac{a_2}{A}\right)^{\alpha}\left(\frac{b_2}{B}\right)^{\beta}\cdots\left(\frac{l_2}{L}\right)^{\lambda}+}{\cdots + \left(\frac{a_n}{A}\right)^{\alpha}\left(\frac{b_n}{B}\right)^{\beta}\cdots\left(\frac{l_n}{L}\right)^{\lambda}}}{A^{\alpha}B^{\beta}\cdots L^{\lambda}}\leq \alpha+\beta +\cdots+\lambda}$$Since $ \alpha+\beta +\cdots+\lambda=1$ we can write $$\splitdfrac{\bigg(\dfrac{a_1}{A}\bigg)^{\alpha}\bigg(\dfrac{b_1}{B}\bigg)^{\beta}\cdots\bigg(\dfrac{l_1}{L}\bigg)^{\lambda} +  \bigg(\dfrac{a_2}{A}\bigg)^{\alpha}\bigg(\dfrac{b_2}{B}\bigg)^{\beta}\cdots\bigg(\dfrac{l_2}{L}\bigg)^{\lambda}+}{\cdots + \bigg(\dfrac{a_n}{A}\bigg)^{\alpha}\bigg(\dfrac{b_n}{B}\bigg)^{\beta}\cdots\bigg(\dfrac{l_n}{L}\bigg)^{\lambda}\leq A^{\alpha}B^{\beta}\cdots L^{\lambda}}$$or 
\begin{multline*}
\boldsymbol{a_{1}^{\alpha} b_{1}^{\beta} \cdots l_{1}^{\lambda}+a_{2}^{\alpha} b_{2}^{\beta} \cdots l_{2}^{\lambda}+\cdots + a_{n}^{\alpha} b_{n}^{\beta} \cdots l_{n}^{\lambda}\leq }\\
\boldsymbol{  \left( a_{1}+\cdots+a_{n} \right)^{\alpha} \left( b_{1}+\cdots +b_{n}\right)^{\beta} \cdots \left(l_{1}+l_{2}+\cdots+l_{n}\right)^{\lambda} }
\end{multline*}
This completes the proof
\pagebreak
\section{Example: Part of An Inequality Proposed by Arqady}
If $a,b,c>0$ and $k \geq\ 0$ then prove that $$ \sum \limits_{cyc}\sqrt{\dfrac{a}{b+kc}}\geq \frac{3}{\sqrt{k+1}} $$ when $a+b+c\geq 3$
Using H\"{o}lder Inequality we get 
\begin{align*}
& \left(\sum \limits_{cyc}\sqrt{\dfrac{a}{b+kc}} \right)^{\frac{2}{3}}\left(\sum \limits_{cyc}\ (b+kc)\right)^{\frac{1}{3}}\geq (a+b+c)\\
\implies &\left(\sum \limits_{cyc}\sqrt{\dfrac{a}{b+kc}} \right)^2 \geq \dfrac{(a+b+c)^3}{\left(\sum \limits_{cyc}\ (b+kc)\right)}=\dfrac{(a+b+c)^2}{k+1}
\end{align*}Hence if $a+b+c\geq 3$ then $$\sum \limits_{cyc}\sqrt{\dfrac{a}{b+kc}}\geq \dfrac{3}{\sqrt{k+1}}$$This completes the proof

\pagebreak

\section{Example: IMO 2001 P2}
Let $a,b,c$ be positive real numbers. Prove that$$\frac{a}{\sqrt{a^2+8bc}}+\frac{b}{\sqrt{b^2+8ca}}+\frac{c}{\sqrt{c^2+8ab}}\geq 1$$
By H\"{o}lder Inequality
\begin{align*}
& \left(\sum_{cyc}\frac{a}{\sqrt{a^2+8bc}}\right)^{\frac{2}{3}}\left(\sum_{cyc}a(a^2+8bc\right)^{\frac{1}{3}}\geq (a+b+c)\\
\implies & \left(\sum_{cyc}\frac{a}{\sqrt{a^2+8bc}}\right)^2\geq \frac{(a+b+c)^3}{a^3+b^3+c^3+24abc)}\\
\end{align*}
Thus it suffices to show that
$$(a+b+c)^{3}\ge a^{3}+b^{3}+c^{3}+24abc$$
Now,$$(a+b+c)^3=\left(\sum_{cyc}a^3 \right)+\left(\sum_{cyc}(3x^2y+3xy^2)\right) +6abc$$ $$\geq a^3+b^3+c^3+18abc+6abc =a^3+b^3+c^3+24abc$$
This completes the proof





\end{document}
